theories/common/Events.v
@@ -317,8 +317,8 @@ Section MASK.
       match e with
       | inl1 _ => true
       | inr1 (inl1 _) => true
-      | inr1 (inr1 (inl1 (SPut k v))) => decide (k ∈ scp)
-      | inr1 (inr1 (inl1 (SGet k))) => decide (k ∈ scp)
+      | inr1 (inr1 (inl1 (SPut k v))) => decide (k.1 ∈ scp)
+      | inr1 (inr1 (inl1 (SGet k))) => decide (k.1 ∈ scp)
       | inr1 (inr1 (inr1 _)) => true
       end.
 
